tests/lean/run/heqSubst.lean
@@ -1,0 +1,3 @@
+example (f : α → α) (a b : α) (h : HEq a b) : f a = f b := by
+  subst h
+  rfl
